modified pad for pull req

Pad.v
@@ -3,10 +3,11 @@ Require Export Quantum.
 Require Export Init.Datatypes.
 Require Export Coq.Sorting.Permutation.
 Require Export Coq.Lists.List.
-
 (** This file provides padding functions to extend a matrix to a larger space.
    This is useful for describing the effect of 1- and 2-qubit gates on a larger
    quantum space. *)
+
+(* if_matrix notation + lemmas *)
 
 Definition if_matrix {n} (b : bool) (u1 u2 : Square n) : Square n :=
   if b then u1 else u2.
@@ -26,8 +27,73 @@ Proof.
 Qed.
 
 #[export] Hint Resolve WF_if_matrix : wf_db.
-(* converting this to if_matrix format results in WF_Matrix Zero not being solved by
-auto with wf_db ?? *)
+
+Definition pad {n} (start dim : nat) (A : Square (2^n)) : Square (2^dim) :=
+  if start + n <=? dim then I (2^start) ⊗ A ⊗ I (2^(dim - (start + n))) else Zero.
+
+Lemma WF_pad : forall n start dim (A : Square (2^n)),
+  WF_Matrix A ->
+  WF_Matrix (pad start dim A).
+Proof.
+  intros n start dim A WFA. unfold pad.
+  bdestruct (start + n <=? dim); auto with wf_db.
+Qed.  
+
+Lemma pad_mult : forall n dim start (A B : Square (2^n)),
+  pad start dim A × pad start dim B = pad start dim (A × B).
+Proof.
+  intros.
+  unfold pad.
+  gridify.
+  reflexivity.
+Qed.
+
+Lemma pad_id : forall n dim,
+  (n < dim)%nat -> @pad 1 n dim (I 2) = I (2 ^ dim).
+Proof. intros. unfold pad. gridify. reflexivity. Qed.
+
+Definition pad_u (dim n : nat) (u : Square 2) : Square (2^dim) := @pad 1 n dim u.
+
+Definition pad_ctrl (dim m n: nat) (u: Square 2) :=
+  if (m <? n) then
+    @pad (1+(n-m-1)+1) m dim (∣1⟩⟨1∣ ⊗ I (2^(n-m-1)) ⊗ u .+ ∣0⟩⟨0∣ ⊗ I (2^(n-m-1)) ⊗ I 2)
+  else if (n <? m) then
+    @pad (1+(m-n-1)+1) n dim (u ⊗ I (2^(m-n-1)) ⊗ ∣1⟩⟨1∣ .+ I 2 ⊗ I (2^(m-n-1)) ⊗ ∣0⟩⟨0∣)
+  else
+    Zero.
+
+(* also possible to define this in terms of pad directly *)
+Definition pad_swap (dim m n: nat) :=
+  pad_ctrl dim m n σx × pad_ctrl dim n m σx × pad_ctrl dim m n σx.
+
+(** Well-formedness *)
+
+Lemma WF_pad_u : forall dim n u, WF_Matrix u -> WF_Matrix (pad_u dim n u).
+Proof.
+  intros. 
+  unfold pad_u.
+  apply WF_pad; easy.
+Qed.
+
+Lemma WF_pad_ctrl : forall dim m n u, WF_Matrix u -> WF_Matrix (pad_ctrl dim m n u).
+  intros. 
+  unfold pad_ctrl.
+  assert (H' : forall n, (2 * 2 ^ n * 2 = 2 ^ (1 + n + 1))%nat).
+  { intros.
+    do 2 rewrite Nat.pow_add_r, Nat.pow_1_r; easy. }
+  bdestruct (m <? n); bdestruct (n <? m); try lia; auto with wf_db.
+  all : apply WF_pad; rewrite H'; apply WF_plus; auto with wf_db.
+Qed.
+
+Lemma WF_pad_swap : forall dim m n, WF_Matrix (pad_swap dim m n).
+  intros.
+  unfold pad_swap.
+  repeat apply WF_mult; apply WF_pad_ctrl; apply WF_σx.
+Qed.
+
+#[export] Hint Resolve WF_pad WF_pad_u WF_pad_ctrl WF_pad_swap : wf_db.
+
+(* Pad2, embed definition + lemmas about commutation *)
 Definition pad2 {dim : nat} (A : Square 2) (i : nat) : Square (2^dim) :=
   if (i <? dim) then (I (2^i) ⊗ A ⊗ I (2^(dim - i - 1))) else Zero.
 
@@ -40,11 +106,12 @@ Qed.
 
 #[export] Hint Resolve WF_pad2 : wf_db.
 
-Fixpoint embed2 {dim : nat} (lp : (list ((Square 2) * nat))) : Square (2^dim)  :=
+Fixpoint embed {dim : nat} (lp : (list ((Square 2) * nat))) : Square (2^dim)  :=
   match lp with
-  | (A, i) :: lp' => @Mmult (2^dim) (2^dim) (2^dim) (@pad2 dim A i) (embed2 lp')
+  | (A, i) :: lp' => @Mmult (2^dim) (2^dim) (2^dim) (@pad2 dim A i) (embed lp')
   | _         => I (2^dim)
   end.
+
 
 Lemma pad2_commutes : forall (A B : Square 2) (i j dim : nat),
 i <> j ->
@@ -56,40 +123,40 @@ Proof.
   gridify; trivial.
   Qed.
 
-Lemma WF_embed2 : forall (dim : nat) (lp : (list ((Square 2) * nat))),
+Lemma WF_embed : forall (dim : nat) (lp : (list ((Square 2) * nat))),
 Forall WF_Matrix (map fst lp) -> 
 NoDup (map snd lp) ->
 Forall (fun n => (n < dim)%nat) (map snd lp) ->
-WF_Matrix (@embed2 dim lp).
+WF_Matrix (@embed dim lp).
 intros. induction lp. 
-+ unfold embed2; auto with wf_db.
++ unfold embed; auto with wf_db.
 + destruct a. bdestruct (n <? dim); Msimpl; auto with wf_db.
   - inversion H; subst. inversion H0; subst. inversion H1; subst.
    simpl. apply WF_mult; auto with wf_db.
   - inversion H1; subst. lia.
 Qed.
 
-#[export] Hint Resolve WF_embed2 : wf_db.
+#[export] Hint Resolve WF_embed : wf_db.
 
-Lemma embed2_commutes_base : forall (i j dim : nat)(A B : Square 2) 
+Lemma embed_commutes_base : forall (i j dim : nat)(A B : Square 2) 
 (lp : (list ((Square 2) * nat))),
   i <> j ->
   WF_Matrix A ->
   WF_Matrix B ->
   (i < dim)%nat ->
   (j < dim)%nat ->
-  @embed2 dim ((A, i) :: (B, j) :: lp) = @embed2 dim ((B, j) :: (A, i) :: lp).
+  @embed dim ((A, i) :: (B, j) :: lp) = @embed dim ((B, j) :: (A, i) :: lp).
   Proof.
     intros. simpl. rewrite <- Mmult_assoc. rewrite pad2_commutes; trivial.
     apply Mmult_assoc.
   Qed.
 
-Lemma embed2_commutes : forall (dim : nat) (lp1 lp2 : list ((Square 2) * nat)),
+Lemma embed_commutes : forall (dim : nat) (lp1 lp2 : list ((Square 2) * nat)),
   Forall WF_Matrix (map fst lp1) ->
   NoDup (map snd lp1) ->
   Forall (fun n => (n < dim)%nat) (map snd lp1) ->
   Permutation lp1 lp2 ->
-  @embed2 dim lp1 = @embed2 dim lp2.
+  @embed dim lp1 = @embed dim lp2.
   Proof.
     intros. induction H2; trivial.
     + simpl. rewrite IHPermutation; trivial. 
@@ -97,7 +164,7 @@ Lemma embed2_commutes : forall (dim : nat) (lp1 lp2 : list ((Square 2) * nat)),
       auto.
       - inversion H0; auto.
       - simpl in H1. rewrite Forall_cons_iff in H1. apply H1.
-    + destruct x, y. apply embed2_commutes_base.
+    + destruct x, y. apply embed_commutes_base.
       - simpl in H0. inversion H0; subst. simpl in *. intros n0eqn. apply H4. auto.
       - simpl in *. inversion H; subst.
       auto.
@@ -112,20 +179,37 @@ Lemma embed2_commutes : forall (dim : nat) (lp1 lp2 : list ((Square 2) * nat)),
       - eapply Permutation_Forall; eauto.
     Qed.
 
+Lemma embed_mult : forall (dim : nat) (lp1 lp2 : list ((Square 2) * nat)),
+Forall WF_Matrix (map fst lp1) ->
+Forall WF_Matrix (map fst lp2) ->
+NoDup (map snd lp1) ->
+NoDup (map snd lp2) ->
+Forall (fun n : nat => (n < dim)%nat) (map snd lp1) ->
+Forall (fun n : nat => (n < dim)%nat) (map snd lp2) ->
+@embed dim lp1 × @embed dim lp2 = @embed dim (lp1 ++ lp2).
+Proof.
+  intros. induction lp1.
+  + simpl. apply Mmult_1_l. apply WF_embed; trivial.
+  + simpl. rewrite <- IHlp1. destruct a. apply Mmult_assoc.
+  inversion H; auto.
+  inversion H1; auto.
+  inversion H3; auto.
+Qed.
+
 (* TODO: find function in stdlib *) 
 Definition abs_diff (a b : nat) := Nat.max (a - b) (b - a).
 
-Definition pad_ctrl (dim m n : nat) (u : Square 2) : Square (2^dim)%nat :=
+Definition pad2_ctrl (dim m n : nat) (u : Square 2) : Square (2^dim)%nat :=
   if m =? n then Zero
   else
     let b := m <? n in
     let μ := min m n in
     let δ := abs_diff m n in
-    (@embed2 dim
+    (@embed dim
     ([((∣1⟩⟨1∣ <|b|> u), μ)] ++
     [((u <|b|> ∣1⟩⟨1∣), (μ + δ)%nat)])) 
     .+ 
-    (@embed2 dim
+    (@embed dim
     ([((∣0⟩⟨0∣ <|b|> I 2), μ)] ++
     [((I 2 <|b|> ∣0⟩⟨0∣), (μ + δ)%nat)])).
 
@@ -158,50 +242,62 @@ Ltac rem_max_min :=
     rewrite Max.max_l by lia 
   end.
 
-Definition pad_u (dim n : nat) (u : Square 2) : Square (2^dim) := @pad2 dim u n.
+Definition pad2_u (dim n : nat) (u : Square 2) : Square (2^dim) := @embed dim [(u,n)].
 
-(* also possible to define this in terms of pad directly *)
-Definition pad_swap (dim m n: nat) :=
-  pad_ctrl dim m n σx × pad_ctrl dim n m σx × pad_ctrl dim m n σx.
+(* also possible to define this in terms of pad2 directly *)
+Definition pad2_swap (dim m n: nat) :=
+  pad2_ctrl dim m n σx × pad2_ctrl dim n m σx × pad2_ctrl dim m n σx.
 
 (** Well-formedness *)
 
-Lemma WF_pad_u : forall dim n u, WF_Matrix u -> WF_Matrix (pad_u dim n u).
+Lemma WF_pad2_u : forall dim n u, WF_Matrix u -> WF_Matrix (pad2_u dim n u).
 Proof.
   intros. 
-  unfold pad_u.
+  unfold pad2_u.
+  unfold embed.
   auto with wf_db. 
 Qed.
 
-Lemma WF_pad_ctrl : forall dim m n u, WF_Matrix u -> WF_Matrix (pad_ctrl dim m n u).
+Lemma WF_pad2_ctrl : forall dim m n u, WF_Matrix u -> WF_Matrix (pad2_ctrl dim m n u).
 Proof.
   intros dim m n u WF_u.
-  unfold pad_ctrl, abs_diff. bdestruct_all; simpl; rem_max_min;
+  unfold pad2_ctrl, abs_diff. bdestruct_all; simpl; rem_max_min;
   restore_dims; auto with wf_db.
   Qed.
 
 
-Lemma WF_pad_swap : forall dim m n, WF_Matrix (pad_swap dim m n).
+Lemma WF_pad2_swap : forall dim m n, WF_Matrix (pad2_swap dim m n).
   intros.
-  unfold pad_swap.
-  repeat apply WF_mult; apply WF_pad_ctrl; apply WF_σx.
+  unfold pad2_swap.
+  repeat apply WF_mult; apply WF_pad2_ctrl; apply WF_σx.
 Qed.
 
-#[export] Hint Resolve WF_pad2 WF_pad_u WF_pad_ctrl WF_pad_swap : wf_db.
+#[export] Hint Resolve WF_pad2 WF_pad2_u WF_pad2_ctrl WF_pad2_swap : wf_db.
+
+(* tactics for NoDup *)
+Ltac NoDupity :=
+  repeat match goal with
+  | |- NoDup [?a] => repeat constructor; auto
+  | |- NoDup _=> repeat constructor; intros []; try lia; auto
+  | [ H1: In ?a ?b |- False ] => inversion H1; auto
+  end.
 
 (* Lemmas about commutativity *)
 
-Lemma pad_A_B_commutes : forall dim m n A B,
+Lemma pad2_A_B_commutes : forall dim m n A B,
   m <> n ->
   (m < dim)%nat ->
   (n < dim)%nat ->
   WF_Matrix A ->
   WF_Matrix B ->
-  pad_u dim m A × pad_u dim n B = pad_u dim n B × pad_u dim m A.
+  pad2_u dim m A × pad2_u dim n B = pad2_u dim n B × pad2_u dim m A.
 Proof.
-  intros. unfold pad_u. unfold WF_Matrix in *.
-   apply pad2_commutes; trivial.
+  intros. unfold pad2_u. unfold WF_Matrix in *.
+  repeat rewrite embed_mult. apply embed_commutes.
+  all : simpl; try auto with wf_db; NoDupity.
+  constructor.
 Qed.
+
 
 Ltac comm_pad2 :=
   repeat match goal with
@@ -211,14 +307,12 @@ Ltac comm_pad2 :=
         | context[pad2 Z z × pad2 X x × pad2 Y y] =>
           try rewrite (pad2_commutes Z X z x dim); 
           try rewrite <- (Mmult_assoc (pad2 X x) (pad2 Z z) (pad2 Y y));
-          try rewrite (pad2_commutes Y Z y z dim);
-          try auto with wf_db
+          try rewrite (pad2_commutes Y Z y z dim)
         | context[pad2 Y y × pad2 Z z × pad2 X x] =>
           try rewrite (Mmult_assoc (pad2 Y y) (pad2 Z z) (pad2 X x));
           try rewrite (pad2_commutes Z X z x dim);
           try rewrite <- (Mmult_assoc (pad2 Y y) (pad2 X x) (pad2 Z z));
-          try rewrite (pad2_commutes Y X y x dim);
-          try auto with wf_db
+          try rewrite (pad2_commutes Y X y x dim)
         end
       | context[@pad2 ?dim ?X ?x × (@pad2 ?dim ?Y ?y × @pad2 ?dim ?Z ?z)] => 
         rewrite <- (Mmult_assoc (pad2 X x) (pad2 Y y) (pad2 Z z))
@@ -226,10 +320,7 @@ Ltac comm_pad2 :=
     end.
 
 
-(* × associates to the left *)
-
-(* convert from pad2 a * pad2 b to embed2 *)
-Lemma pad_A_ctrl_commutes : forall dim m n o A B,
+Lemma pad2_A_ctrl_commutes : forall dim m n o A B,
   m <> n ->
   m <> o ->
   (m < dim)%nat ->
@@ -237,41 +328,38 @@ Lemma pad_A_ctrl_commutes : forall dim m n o A B,
   (o < dim)%nat ->
   WF_Matrix A ->
   WF_Matrix B ->
-  pad_u dim m A × pad_ctrl dim n o B = pad_ctrl dim n o B × pad_u dim m A.
+  pad2_u dim m A × pad2_ctrl dim n o B = pad2_ctrl dim n o B × pad2_u dim m A.
 Proof.
-  intros. unfold pad_u, pad_ctrl, abs_diff. simpl. bdestruct_all; simpl; rem_max_min;
+  Opaque embed.
+  intros. unfold pad2_u, pad2_ctrl, abs_diff. bdestruct_all; simpl; rem_max_min;
   Msimpl; trivial.
-  + repeat rewrite Mmult_plus_distr_l. rewrite Mmult_plus_distr_r. 
-  replace (n + (o - n))%nat with o by lia. 
-  comm_pad2.
-  + repeat rewrite Mmult_plus_distr_r. rewrite Mmult_plus_distr_l.
-  replace (o + (n - o))%nat with n by lia.
-  comm_pad2.
-Qed.
+  + repeat rewrite Mmult_plus_distr_l; repeat rewrite Mmult_plus_distr_r.
+  rewrite le_plus_minus_r by (apply Nat.lt_le_incl; trivial).
+  repeat rewrite embed_mult; simpl.
+  rewrite (embed_commutes dim [(A, m); (∣1⟩⟨1∣, n); (B, o)] [(∣1⟩⟨1∣, n); (B, o); (A, m)]).
+  rewrite (embed_commutes dim [(A, m); (∣0⟩⟨0∣, n); (I 2, o)] [(∣0⟩⟨0∣, n); (I 2, o); (A, m)]).
+  trivial.
+  all : simpl; NoDupity; auto with wf_db. 
+  all : rewrite perm_swap; apply perm_skip; apply perm_swap.
 
-(* Everything after here is a WIP wrt writing it in terms of embed2 *)
+  + repeat rewrite Mmult_plus_distr_l; repeat rewrite Mmult_plus_distr_r.
+  rewrite le_plus_minus_r by trivial; repeat rewrite embed_mult; simpl.
+  rewrite (embed_commutes dim [(A, m); (B, o); (∣1⟩⟨1∣, n)] [(B, o); (∣1⟩⟨1∣, n); (A, m)]).
+  rewrite (embed_commutes dim [(A, m); (I 2, o); (∣0⟩⟨0∣, n)] [(I 2, o); (∣0⟩⟨0∣, n); (A, m)]).
+  trivial.
+  all : simpl; NoDupity; auto with wf_db.
+  all : rewrite perm_swap; apply perm_skip; apply perm_swap.
+  Qed.
 
 (** Unitarity *)
 
-(* if i < dim and u is a wf unitary matrix, then  *)
-(* Lemma pad_unitary : forall n (u : Square (2^n)) i dim,
-(i < dim)%nat ->
-WF_Unitary u ->
-WF_Unitary  *)
-
-(* 
-Lemma pad_unitary : forall n (u : Square (2^n)) i dim,
-    (i < dim)%nat -> 
+Lemma pad_unitary : forall n (u : Square (2^n)) start dim,
+    (start + n <= dim)%nat -> 
     WF_Unitary u ->
-    WF_Unitary (@pad2 dim u i).
+    WF_Unitary (pad start dim u).
 Proof.
-  intros n u i dim lt_con [WF U_u].
-  split.
-  apply WF_pad2.
-  apply WF.
-  auto with wf_db.
-  apply WF_pad2. apply WF.
-  apply WF_pad; auto.
+  intros n u start dim B [WF U].
+  split. apply WF_pad; auto.
   unfold pad.
   gridify.
   Msimpl.
@@ -284,47 +372,6 @@ Lemma pad_u_unitary : forall dim n u,
     WF_Unitary u ->
     WF_Unitary (pad_u dim n u).
 Proof. intros. apply pad_unitary. lia. auto. Qed.  
-
-Lemma pad_ctrl'_unitary : forall dim m n u,
-m <> n -> 
-(m < dim)%nat ->
-(n < dim)%nat ->
-WF_Unitary u ->
-WF_Unitary (pad_ctrl' dim m n u).
-Proof.
-  intros dim m n u neq_mn lm ln wfu.
-  destruct wfu.
-  unfold pad_ctrl', pad, WF_Unitary. bdestruct_all; simpl; try auto with wf_db.
-  + replace (Init.Nat.min m n) with m in * by lia; split; restore_dims.
-    - apply WF_kron; auto with wf_db.
-    - Msimpl; unfold abs_diff;
-    replace (Init.Nat.max (m - n) (n - m)) with ((n - m)%nat) by lia;
-    gridify; rewrite H0; Qsimpl;
-    replace (m + 1 + d + 1 + x - (m + S (d + 1)))%nat with x by lia;
-    repeat rewrite kron_assoc; try auto with wf_db;
-    repeat rewrite id_kron; restore_dims;
-    rewrite <- kron_plus_distr_l; rewrite <- kron_plus_distr_r;
-    rewrite Mplus10; repeat rewrite id_kron; reflexivity.
-  + split; restore_dims.
-    - auto with wf_db.
-    - unfold abs_diff in H2; gridify.
-  + replace (Init.Nat.min m n) with n by lia; unfold abs_diff;
-  replace (Init.Nat.max (m - n)(n - m)) with (m - n)%nat by lia.
-  split; restore_dims.
-    - apply WF_kron; auto with wf_db.
-    - Msimpl; gridify; Qsimpl; rewrite H0; 
-    replace (n + 1 + x1 - n - 1)%nat with x1 by lia;
-    repeat rewrite <- kron_assoc; try auto with wf_db;
-    repeat rewrite id_kron; restore_dims;
-    rewrite <- kron_plus_distr_r; rewrite <- kron_plus_distr_l;
-    rewrite Mplus10; repeat rewrite id_kron;
-    replace (n + 1 + (x1 + S x0) - (n + S (x1 + 1)))%nat with x0 by lia; reflexivity.
-  + split; restore_dims.
-  - auto with wf_db.
-  - unfold abs_diff in H2; gridify.
-  Qed.
-
-
 
 Lemma pad_ctrl_unitary : forall dim m n u,
     m <> n ->
@@ -396,42 +443,6 @@ Proof.
   gridify; trivial.
 Qed.
 
-(* theorems and lemmas about diagonalizability of matrices might be helpful
-and make the next two proofs a lot faster.  *)
-
-Lemma pad_A_ctrl'_commutes :  forall dim m n o A B,
-m <> n ->
-m <> o ->
-WF_Matrix A ->
-WF_Matrix B ->
-pad_u dim m A × pad_ctrl' dim n o B = pad_ctrl' dim n o B × pad_u dim m A.
-Proof.
-  intros. unfold pad_ctrl', pad_u, pad, abs_diff.
-  bdestruct_all; try auto with wf_db.
-  - replace (Init.Nat.min n o) with n in * by lia.
-  replace (Init.Nat.max (n - o) (o - n)) with (o - n)%nat in * by lia.
-  replace (n + (1 + (o - n - 1) + 1))%nat with (o + 1)%nat in * by lia.
-  simpl in *. 
-  assert (WF_Diagonal (I (2 ^ m) ⊗ A ⊗ I (2 ^ (dim - (m + 1))))).
-  + unfold WF_Diagonal. split. auto with wf_db.
-  intros. gridify.
-  Admitted.
-
-Lemma pad_ctrl'_ctrl'_commutes : forall dim m n o p A B,
-  m <> o ->
-  m <> p ->
-  n <> o ->
-  n <> p ->
-  WF_Matrix A ->
-  WF_Matrix B ->
-  pad_ctrl_embed dim m n A × pad_ctrl_embed dim o p B = pad_ctrl_embed dim o p B × pad_ctrl_embed dim m n A.
-Proof.
-  intros. unfold pad_ctrl_embed; bdestruct_all; rem_max_min; simpl;
-  repeat rewrite le_plus_minus_r by lia; Msimpl; trivial. 
-
-
-
-
 (* Horribly slow due to many subcases.
    TODO: can we speed this up be tweaking the ordering in gridify? *)
 Lemma pad_ctrl_ctrl_commutes : forall dim m n o p A B,
@@ -445,12 +456,7 @@ Lemma pad_ctrl_ctrl_commutes : forall dim m n o p A B,
 Proof.
   intros.
   unfold pad_ctrl, pad.
-  bdestruct_all.
+  bdestruct_all.  
   all : try rewrite Mmult_0_r; try rewrite Mmult_0_l; try easy.
-  
-  
-
-
-Admitted.
-  (* gridify; trivial. *)
-Qed. *)
+  all : gridify; trivial.
+Qed.
